src/lib/Kernel/Map.v
@@ -17,15 +17,24 @@ Definition all_wall_map (width height : positive) : t width height :=
 
 Program Definition build_horizontal_road
   {width height : positive}
-  (x : HalfOpenRange.t)
   (y : N)
+  (x : HalfOpenRange.t)
   (map : t width height)
-  (x_spec : HalfOpenRange.upper x <= N.pos width)
-  (y_spec : y < N.pos height) : t width height :=
+  (y_spec : y < N.pos height)
+  (x_spec : HalfOpenRange.upper x <= N.pos width) : t width height :=
   NonEmptyArray.map_nth map y (fun row => NonEmptyArray.update_range row x false x_spec) _.
 
+Program Definition build_vertical_road
+  {width height : positive}
+  (y : HalfOpenRange.t)
+  (x : N)
+  (map : t width height)
+  (y_spec : HalfOpenRange.upper y <= N.pos height)
+  (x_spec : x < N.pos width) : t width height :=
+  NonEmptyArray.update_range map y (fun row => NonEmptyArray.update row x false _) _.
+
 Program Definition initial_map : t 80 50 :=
-  build_horizontal_road (HalfOpenRange.make 10 50 _) 25 (all_wall_map 80 50) _ _.
+  build_horizontal_road 25 (HalfOpenRange.make 10 50 _) (all_wall_map 80 50) _ _.
 Next Obligation.
 Proof.
   lia.
